

## Homework 4, Math 4150

1. Exercise Set 3.3, #40 (with some additional parts).

(a) Let  $a \in \mathbb{Z}$  with  $a > 0$ . Use induction to prove that

$$\sum_{m=1}^a m = \frac{a(a+1)}{2},$$

and that

$$\sum_{m=1}^a m^3 = \left( \frac{a(a+1)}{2} \right)^2.$$

**Solution.** First we show,  $\sum_{m=1}^a m = \frac{a(a+1)}{2}$ . Take  $a = 1$  we have  $\sum_{m=1}^1 = 1$  and  $\frac{a(a+1)}{2} = \frac{1(1+1)}{2} = \frac{2}{2} = 1$ . Hence base case is true. Now, assume true for some arbitrary  $n$ , so we have,

$$\sum_{m=1}^n m = \frac{n(n+1)}{2}$$

Now we need to show the case for  $n+1$  is true. First add  $n+1$  to both sides above. We get,

$$\begin{aligned} \left( \sum_{m=1}^n m \right) + (n+1) &= \frac{n(n+1)}{2} + (n+1) \\ \left( \sum_{m=1}^{n+1} m \right) &= (n+1) \left( \frac{n}{2} + 1 \right) \\ &= \frac{(n+1)(n+2)}{2} \end{aligned}$$

which is the case for  $n+1$ . Hence by induction we have  $\sum_{m=1}^a = \frac{a(a+1)}{2}$ .

Now we need to show that  $\sum_{m=1}^a m^3 = \left( \frac{a(a+1)}{2} \right)^2$ . First we verify base case where  $a = 1$  so we have  $\sum_{m=1}^1 m^3 = 1^3 = 1$  and we have  $\left( 1(1+1)\frac{1}{2} \right)^2 = 1^2 = 1$ . So base case is true. Now assume true for case  $a = n$ . So we have,

$$\sum_{m=1}^n m^3 = \left( \frac{n(n+1)}{2} \right)^2$$

Now we need to show case  $a = n + 1$  is true. We add  $(n + 1)^3$  to both sides to get,

$$\begin{aligned}
 \left( \sum_{m=1}^n m^3 \right) (n+1)^3 &= \left( \frac{n(n+1)}{2} \right)^2 + (n+1)^3 \\
 \sum_{m=1}^{n+1} m^3 &= \left( \frac{n(n+1)}{2} \right)^2 + (n+1)^3 \\
 &= (n+1)^2 \left( \left( \frac{n}{2} \right)^2 + (n+1) \right) \\
 &= (n+1)^2 \left( \frac{n^2 + 4n + 4}{2^2} \right) \\
 &= (n+1)^2 \left( \frac{(n+2)^2}{2^2} \right) \\
 &= \left( \frac{(n+1)(n+2)}{2} \right)^2
 \end{aligned}$$

Which is the case for  $n + 1$ . Hence by induction we have  $\sum_{m=1}^a m^3 = \left( \frac{a(a+1)}{2} \right)^2$

(b) Let  $n \in \mathbb{Z}$  with  $n > 0$ . Use the previous part to prove that

$$\left( \sum_{d|n, d>0} v(d) \right)^2 = \sum_{d|n, d>0} (v(d))^3.$$

[Hint: It suffices to prove the equation in (b) for powers of prime numbers (justify this)]

**Solution.** As  $v$  is multiplicative it is enough to show the above for prime powers. So consider  $n = p^a$  we have,

$$\begin{aligned}
 \left( \sum_{d|p^a} v(d) \right)^2 &= (v(p^a) + v(p^{a-1}) + \dots + p + 1)^2 \\
 &= ((a+1) + a + (a-1) + \dots + 2 + 1)^2 \\
 &= \left( \frac{(a+1)(a+2)}{2} \right)^2 \\
 &= \sum_{m=1}^{a+1} m^3 \\
 &= 1^3 + 2^3 + \dots + (a+1)^3 \\
 &= v(1)^3 + v(p)^3 + \dots + v(p^{a-1})^3 + v(p)^3 \\
 &= \sum_{d|p^a, d>0} (v(d))^3
 \end{aligned}$$

Now we justify why the multiplicativity of  $v$  justifies showing only for prime powers. We have  $n = p_1^{a_1} \dots p_n^{a_n}$ . Now if  $d \mid n$  then  $d = p_1^{b_1} \dots p_n^{b_n}$  where  $1 \leq b_k \leq a_k$  so  $v(d) = v(p_1^{b_1}) \dots v(p_n^{b_n})$ . Now,

$$\begin{aligned}
\left( \sum_{d \mid n, d > 0} v(d) \right)^2 &= \left( \sum_{d \mid p_1^{a_1} \dots p_k^{a_k}, d > 0} v(d) \right)^2 \\
&= \left( \sum_{d \mid p_1^{a_1}} v(d) \dots \sum_{d \mid p_k^{a_k}} v(d) \right)^2 \\
&= \left( \sum_{d \mid p_1^{a_1}} v(d) \right)^2 \dots \left( \sum_{d \mid p_k^{a_k}} v(d) \right)^2 \\
&= \sum_{d \mid p_1^{a_1}} (v(d))^3 \dots \sum_{d \mid p_k^{a_k}} (v(d))^3 \\
&= \sum_{d \mid n} (v(d))^3
\end{aligned}$$

true as  $v(d)$  is multiplicative implies that  $v(d)^3$  is also multiplicative.

Blank page:

2. Exercise Set 3.4, #48. Let  $n \in \mathbb{Z}$  with  $n > 0$ . Prove that

$$\frac{\sigma(n!)}{n!} \geq \sum_{i=1}^n \frac{1}{i}.$$

**Solution.**

We know that  $\sigma$  is the sum of divisors. So  $\sigma(n!) = \sigma(1 \cdot 2 \cdots (n-1) \cdot (n))$ . Now note that out of all the divisors of  $n!$  we have  $n!, n!/2, \dots, n!/n$  are all unique divisors of  $n!$ . So  $\sigma(n!)$  is the sum of all divisors, it is at least as big as  $n! + n!/2 \cdots + n!/n$ . Hence we get,

$$\begin{aligned} \sigma(n!) &\geq n! + \frac{n!}{2} + \cdots + \frac{n!}{n} \\ \frac{\sigma(n!)}{n!} &\geq 1 + \frac{1}{2} + \cdots + \frac{1}{n} \\ &= \sum_{i=1}^n \frac{1}{i} \end{aligned}$$

3. Exercise Set 3.5, # 58.

**Definiton:** Let  $k, n \in \mathbb{Z}$  with  $k, n > 1$ . Then  $n$  is said to be  $k$ -perfect if  $\sigma(n) = kn$  (Note: A 2-perfect number is perfect in the usual sense).

- (a) Prove that 120 is 3-perfect.

**Solution.** We have  $120 = 2^3 3^1 5^1$  so we have  $\sigma(120) = \frac{2^4-1}{1} \frac{3^2-1}{2} \frac{5^2-1}{4} = 15 \cdot 4 \cdot 6 = 360 = 3 \cdot 120$  and hence we show it is 3-perfect.

- (b) Find all 3-perfect numbers of the form  $2^k 3p$  where  $p$  is an odd prime number.

**Solution.** For  $2^k 3p$  to be a 3-perfect number we have,

$$\sigma(2^k 3p) = \left( \frac{2^{k+1} - 1}{1} \right) \left( \frac{3^2 - 1}{2} \right) \left( \frac{p^2 - 1}{p - 1} \right) = 2^k 3^2 p$$

And we have,

$$\begin{aligned} \left( \frac{2^{k+1} - 1}{1} \right) \left( \frac{3^2 - 1}{2} \right) \left( \frac{p^2 - 1}{p - 1} \right) &= 2^k 3^2 p \\ (2^{k+1} - 1)(4)(p + 1) &= 2^k 9p \\ \left( 2 - \frac{1}{2^k} \right)(4p + 4) &= 9p \\ 8(p + 1) - \frac{4(p + 1)}{2^k} &= 9p \\ (8 - p)2^k &= 4(p + 1) \end{aligned}$$

We see that  $4(p + 1)$  is positive so  $8 - p > 0$  so  $p < 8$ . The only odd primes smaller than 8 are 3, 5, 7. For each of those numbers we have  $52^k = 4(4)$  clearly does not have a solution for  $k$ . For 5 we have  $3 \cdot 2^k = 4(6)$ . Here  $k = 3$  and for 7 we have  $2^k = 4(8)$  so  $k = 5$ . So we have two numbers,  $2^3 3 \cdot 5 = 120$  and  $2^5 3 \cdot 7 = 672$

- (c) Let  $n \in \mathbb{Z}$  with  $n > 1$  and let  $p$  be a prime number not dividing  $n$ . Prove that if  $n$  is  $p$ -perfect, then  $pn$  is  $(p + 1)$ -perfect.

**Solution.**

We have  $n$  is  $p$  perfect. Let  $n = p_1^{a_1} \dots p_n^{a_n}$  so we have  $\sigma(n) = \sigma(p_1^{a_1}) \dots \sigma(p_n^{a_n}) = \frac{p_1^{a_1+1}-1}{p_1-1} \dots \frac{p_n^{a_n+1}-1}{p_n-1}$ . As  $n$  is  $p$  perfect we have,  $\sigma(n) = pn$ . Now consider  $pn$ . As  $p \nmid n$  we have  $pn = p_1^{a_1} \dots p_n^{a_n} p$ . So we can write,

$$\begin{aligned} \sigma(pn) &= \sigma(p_1^{a_1}) \dots \sigma(p_n^{a_n}) \sigma(p) \\ &= \frac{p_1^{a_1+1} - 1}{p_1 - 1} \dots \frac{p_n^{a_n+1} - 1}{p_n - 1} \frac{p^2 - 1}{p - 1} \\ &= \frac{p_1^{a_1+1} - 1}{p_1 - 1} \dots \frac{p_n^{a_n+1} - 1}{p_n - 1} (p + 1) \\ &= \sigma(n)(p + 1) \\ &= pn(p + 1) \end{aligned}$$

as  $\sigma(n) = pn$ . But this means that we have  $\sigma(pn) = (p + 1)(pn)$  which by definition means that  $pn$  is  $p + 1$ -perfect .

Blank page:

4. Exercise Set 3.6, #65.

**Definiton:** Let  $n \in \mathbb{Z}$  with  $n > 0$ . Von Mangoldt's function, denoted  $\Lambda(n)$ , is given by

$$\Lambda(n) := \begin{cases} \ln p & \text{if } n = p^a \text{ for some } p \text{ prime and } a \in \mathbb{Z} \\ 0 & \text{otherwise} \end{cases}.$$

Prove that

$$\Lambda(n) = - \sum_{d|n, d>0} \mu(d) \ln d.$$

**Solution.**

First trivially if  $n = 1$  we have  $\Lambda(n) = \ln(1) = 0$  and as the only divisor of 1 is itself we have  $-\mu(1) \ln(1) = 0$  and hence we have  $\Lambda(n) = - \sum_{d|n, d>0} \mu(d) \ln d$ .

Now consider if  $n = p_1 \dots p_k$  if  $p_1, \dots, p_k$  are distinct. Then we have  $\Lambda(n) = 0$  if  $k > 1$  else  $\Lambda(n) = \ln(p_1)$ . We have the divisors of  $n$  are  $p_1 \dots p_i$  for  $1 \leq i \leq k$ . For any arbitrary divisors we have  $\mu(d) = \mu(p_1 \dots p_i) = (-1)^i$  and  $\ln(d) = \ln(p_1 \dots p_i) = \ln(p_1) + \dots + \ln(p_i)$ . First, if  $k = 1$  we get the only divisor is  $p_1$  so  $-\sum_{d|n, d>0} \mu(d) \ln(d) = -\mu(p_1) \ln(p_1) = -(-1)^1 \ln(p_1) = \ln(p_1) = \Lambda(n)$ . For  $k > 1$  we get,

$$\begin{aligned} - \sum_{d|n, d>0} \mu(d) \ln d &= - \left( \sum_i \ln(p_i) - \sum_{1 \leq i < j \leq k} \ln(p_i p_j) + \dots (-1)^{k+1} \ln(p_1 \dots p_k) \right) \\ &= - \left( \sum_i \ln(p_i) - \sum_{1 \leq i < j \leq k} (\ln(p_i) + \ln(p_j)) + \dots (-1)^k (\ln(p_1) + \dots + \ln(p_k)) \right) \\ &= 0 \end{aligned}$$

Lastly if  $p^2 \mid n$  for some  $p$  then we have either  $n = p^a$  for  $a \geq 2$  in which case we have  $-\sum \mu(d) \ln(d) = -(\mu(1) \ln(1) + \mu(p) \ln(p) + \dots \mu(p^a) \ln(p^a))$ . But we know that  $\mu(p^a)$  for  $a > 2$  is zero so we get  $-(\mu(1) \ln(1) + \mu(p) \ln(p)) = -(-\ln(p) + 0) = \ln(p)$  which is our desired solution. Now if  $n = p_1^{a_1} \dots p_n^{a_n}$  for all  $a_1 \dots a_n \geq 2$  which is the case where we have some  $p_k^2 \mid n$ . Here note that across all the divisors of  $n$  the ones with power greater than 1 for any of the primes will go to zero in the sum as we have  $\mu(d)$  for that divisor as zero. So the only divisors that remain are  $p_1 \dots p_i$  for  $1 \leq i \leq k$ . Now note that in this case the above expansion will apply and we get the sum as going to zero.



5. Exercise Set 3.6, #69. This exercise presents an interpretation of the Möbius Inversion Formula from the point of view of convolutions.

**Definition:** Let  $n \in \mathbb{Z}$  with  $n > 0$ , and let  $f$  and  $g$  be arithmetic functions. The convolution of  $f$  and  $g$ , denoted  $f \star g$ , is given by

$$(f \star g)(n) := \sum_{d|n, d>0} f(d)g\left(\frac{n}{d}\right).$$

- (a) **Commutativity:** Let  $f$  and  $g$  be arithmetic functions. Prove that  $f \star g = g \star f$ .

**Solution.** We have,

$$\begin{aligned} (f \star g)(n) &= \sum_{d|n, d>0} f(d)g\left(\frac{n}{d}\right) \\ &= \sum_{d|n, d>0} f\left(\frac{n}{d}\right)g(d) \\ &= \sum_{d|n, d>0} g(d)f\left(\frac{n}{d}\right) \\ &= (g \star f)(n) \end{aligned}$$

Hence, it is commutative.

- (b) **Associativity:** Let  $f$ ,  $g$ , and  $h$  be arithmetic functions. Prove that  $(f \star g) \star h = f \star (g \star h)$ .

**Solution.** We have,

$$\begin{aligned} ((f \star g) \star h)(n) &= \sum_{d|n, d>0} (f \star g)(d)h\left(\frac{n}{d}\right) \\ &= \sum_{d|n, d>0} \left( \sum_{e|d, e>0} f(e)g\left(\frac{d}{e}\right) \right) h\left(\frac{n}{d}\right) \\ &= \sum_{d|n, d>0} h\left(\frac{n}{d}\right) \left( \sum_{e|d, e>0} f(e)g\left(\frac{d}{e}\right) \right) \\ &= \sum_{d|n, d>0} h\left(\frac{n}{d}\right) \left( \sum_{e|d, e>0} f\left(\frac{d}{e}\right)g(e) \right) \\ &= \sum_{d|n, d>0} f\left(\frac{n}{d}\right) \left( \sum_{e|d, e>0} h\left(\frac{d}{e}\right)g(e) \right) \\ &= \sum_{d|n, d>0} f(d)(h \star g)\left(\frac{n}{d}\right) \\ &= f \star (g \star h) \end{aligned}$$

(c) **Identity:** For  $n \in \mathbb{Z}$  with  $n > 0$ , let

$$\delta(n) = \begin{cases} 1 & \text{if } n = 1 \\ 0 & \text{otherwise} \end{cases}.$$

Let  $f$  be an arithmetic function. Prove that  $f \star \delta = \delta \star f = f$ .

**Solution.** We have,

$$\begin{aligned} f \star \delta &= \sum_{d|n, d>0} f(d) \delta\left(\frac{n}{d}\right) \\ &= \sum_{d|n, d>0} f\left(\frac{n}{d}\right) \delta(d) \end{aligned}$$

Note that for all divisors except 1 we have  $\delta(d) = 0$ , so in our summation all the terms except for when  $d = 1$  will go to zero so we get,

$$\begin{aligned} (f \star \delta)(n) &= f(1)\delta(n) + \cdots + f(n)\delta(1) \\ &= 0 + \cdots + f(n)\delta(1) \\ &= f(n) \cdot 1 \\ &= f(n) \end{aligned}$$

So we have  $f \star \delta = f$ . Now as we showed commutativity in (a) we have  $f \star \delta = \delta \star f$  and hence we have  $f \star \delta = \delta \star f = f$

(d) **Inverses:** For  $n \in \mathbb{Z}$  with  $n > 0$ , let  $\mathbf{1}(n) = 1$ . In other words,  $\mathbf{1}$  is the arithmetic function mapping every positive integer to 1. Prove that  $\mu \star \mathbf{1} = \mathbf{1} \star \mu = \delta$ .

**Solution.**

We have,

$$\begin{aligned} \mu \star \mathbf{1} &= \sum_{d|n, d>0} \mu(d) \mathbf{1}\left(\frac{n}{d}\right) \\ &= \sum_{d|n, d>0} \mu(d) \end{aligned}$$

Now the right term, by Proposition 3.14 is,

$$\sum_{d|n, d>0} \mu(d) = \begin{cases} 1, & \text{if } n = 1 \\ 0, & \text{otherwise} \end{cases} = \delta(n)$$

Hence, we have  $\mu \star \mathbf{1} = \delta$  and because of commutativity we also have  $\mu \star \mathbf{1} = \mathbf{1} \star \mu = \delta$

(e) **Möbius Inversion Formula:** Prove the Möbius Inversion Formula using convolutions.

[Hint: Theorem 3.5 can be restated as  $f = g \star \mathbf{1}$  if and only if  $g = \mu \star f = f \star \mu$ .]

**Solution.**

( $\Rightarrow$ ) We have  $f(n) = \sum_{d|n, d>0} g(d)$  which is equivalent to  $f = g \star \mathbf{1}$ . Now using the above properties we have,

$$\begin{aligned} f &= g \star \mathbf{1} \\ f \star \mu &= (g \star \mathbf{1}) \star \mu \\ f \star \mu &= g \star (\mathbf{1} \star \mu) && \text{using associativity} \\ f \star \mu &= g \star \delta && \text{using (d)} \\ f \star \mu &= g && \text{using (c)} \end{aligned}$$

As we have commutativity, we now have  $g = f \star \mu = \mu \star f$

( $\Leftarrow$ )

Now assume we have  $g = f \star \mu = \mu \star f$  then we can write,

$$\begin{aligned} g &= f \star \mu \\ g \star \mathbf{1} &= (f \star \mu) \star \mathbf{1} \\ g \star \mathbf{1} &= f \star (\mu \star \mathbf{1}) \\ g \star \mathbf{1} &= f \star (\delta) \\ g \star \mathbf{1} &= f \end{aligned}$$

So we get  $f = g \star \mathbf{1}$  which is our solution.

Blank page: